Final pairing low equiv mid

src/specs/FinalPairing.ec
@@ -1,3 +1,5 @@
+pragma Goals:printall.
+
 require        Constants.
 require import Field.
 require import PointMulAndAddIntoDest.
@@ -9,6 +11,8 @@ require import Utils.
 require import Verifier.
 require import VerifierConsts.
 require import YulPrimops.
+
+import MemoryMap.
 
 module FinalPairing = {
   proc low(): unit = {
@@ -33,7 +37,7 @@ module FinalPairing = {
       PointMulAndAddIntoDest.low(PROOF_RECURSIVE_PART_P1_X_SLOT, uu, PAIRING_PAIR_WITH_GENERATOR_X_SLOT);
       PointMulAndAddIntoDest.low(PROOF_RECURSIVE_PART_P2_X_SLOT, uu, PAIRING_PAIR_WITH_X_X_SLOT);
     }
-    
+
     _20 <@ Primops.mload(PAIRING_PAIR_WITH_GENERATOR_X_SLOT);
     Primops.mstore(W256.zero, _20);
     _23 <@ Primops.mload(PAIRING_PAIR_WITH_GENERATOR_Y_SLOT);
@@ -52,6 +56,7 @@ module FinalPairing = {
     Primops.mstore(W256.of_int 352, VerifierConsts.G2_ELEMENTS_1_Y2);
     _47 <@ Primops.gas();
     success <@ Primops.staticcall(_47, W256.of_int 8, W256.zero, W256.of_int 384, W256.zero, W256.of_int 32);
+    
     if (bool_of_uint256 (PurePrimops.iszero success))
     {
       RevertWithMessage.low(W256.of_int 32, W256.of_int STRING (*finalPairing: precompile failure*));
@@ -62,6 +67,68 @@ module FinalPairing = {
     {
       RevertWithMessage.low(W256.of_int 29, W256.of_int STRING (*finalPairing: pairing failure*));
     }
+  }
+
+  proc mid(u: int, z: int, pairing_pair_with_generator: (int*int), pairing_buffer_point: (int*int), opening_proof_at_z: (int*int), opening_proof_at_z_omega: (int*int), vk_recursive_flag: bool, recursive_part_p1: (int*int), recursive_part_p2: (int*int)): bool = {
+    var _5, zOmega, uu;
+    var pairing_pair_with_x: (int*int);
+    var pairing_pair_with_generator_opt, pairing_pair_with_x_opt: (int*int) option;
+    var pairing_result: bool option;
+    var failed: bool;
+    failed <- false;
+    _5 <- z;
+    zOmega <- (_5 * Constants.OMEGA) %% Constants.R;
+
+    pairing_pair_with_generator_opt <@ PointSubAssign.mid(pairing_pair_with_generator, pairing_buffer_point);
+    failed <- failed \/ is_none pairing_pair_with_generator_opt;
+    pairing_pair_with_generator <- odflt (0,0) pairing_pair_with_generator_opt;
+
+    pairing_pair_with_generator_opt <@ PointMulAndAddIntoDest.mid(opening_proof_at_z.`1, opening_proof_at_z.`2, z, pairing_pair_with_generator.`1, pairing_pair_with_generator.`2);
+    failed <- failed \/ is_none pairing_pair_with_generator_opt;
+    pairing_pair_with_generator <- odflt (0,0) pairing_pair_with_generator_opt;
+
+    pairing_pair_with_generator_opt <@ PointMulAndAddIntoDest.mid(opening_proof_at_z_omega.`1, opening_proof_at_z_omega.`2, (zOmega * u) %% Constants.R, pairing_pair_with_generator.`1, pairing_pair_with_generator.`2);
+    failed <- failed \/ is_none pairing_pair_with_generator_opt;
+    pairing_pair_with_generator <- odflt (0,0) pairing_pair_with_generator_opt;
+
+    pairing_pair_with_x_opt <@ PointMulAndAddIntoDest.mid(opening_proof_at_z_omega.`1, opening_proof_at_z_omega.`2, u, opening_proof_at_z.`1, opening_proof_at_z.`2);
+    failed <- failed \/ is_none pairing_pair_with_x_opt;
+    pairing_pair_with_x <- odflt (0,0) pairing_pair_with_x_opt;
+
+    pairing_pair_with_x_opt <@ PointNegate.mid(pairing_pair_with_x);
+    failed <- failed \/ is_none pairing_pair_with_x_opt;
+    pairing_pair_with_x <- odflt (0,0) pairing_pair_with_x_opt;
+
+    if (vk_recursive_flag)
+    {
+      uu <- (u * u) %% Constants.R;
+      pairing_pair_with_generator_opt <@ PointMulAndAddIntoDest.mid(recursive_part_p1.`1, recursive_part_p1.`2, uu, pairing_pair_with_generator.`1, pairing_pair_with_generator.`2);
+      failed <- failed \/ is_none pairing_pair_with_generator_opt;
+      pairing_pair_with_generator <- odflt (0,0) pairing_pair_with_generator_opt;
+
+      pairing_pair_with_x_opt <@ PointMulAndAddIntoDest.mid(recursive_part_p2.`1, recursive_part_p2.`2, uu, pairing_pair_with_x.`1, pairing_pair_with_x.`2);
+      failed <- failed \/ is_none pairing_pair_with_x_opt;
+      pairing_pair_with_x <- odflt (0,0) pairing_pair_with_x_opt;
+    }
+    
+    pairing_result <- ecPairing_precompile
+      (
+        (FieldQ.inF pairing_pair_with_generator.`1, FieldQ.inF pairing_pair_with_generator.`2),
+        (
+          (FieldQ.inF Constants.G2_ELEMENT_0.`1.`1, FieldQ.inF Constants.G2_ELEMENT_0.`1.`2),
+          (FieldQ.inF Constants.G2_ELEMENT_0.`2.`1, FieldQ.inF Constants.G2_ELEMENT_0.`2.`2)
+        )
+      )
+      (
+        (FieldQ.inF pairing_pair_with_x.`1, FieldQ.inF pairing_pair_with_x.`2),
+        (
+          (FieldQ.inF Constants.G2_ELEMENT_1.`1.`1, FieldQ.inF Constants.G2_ELEMENT_1.`1.`2),
+          (FieldQ.inF Constants.G2_ELEMENT_1.`2.`1, FieldQ.inF Constants.G2_ELEMENT_1.`2.`2)
+        )
+      );
+    failed <- failed \/ !(odflt false pairing_result);
+
+    return !failed;
   }
 }.
 
@@ -149,3 +216,1359 @@ lemma finalPairing_extracted_equiv_low:
       call revertWithMessage_extracted_equiv_low. skip. by progress.
       skip. by progress.*)
     qed.
+
+lemma finalPairing_low_equiv_mid:
+    equiv [
+      FinalPairing.low ~ FinalPairing.mid:
+      !Primops.reverted{1} /\
+      u{2} = W256.to_uint (load Primops.memory{1} STATE_U_SLOT) /\
+      z{2} = W256.to_uint (load Primops.memory{1} STATE_Z_SLOT) /\
+      pairing_pair_with_generator{2}.`1 = W256.to_uint (load Primops.memory{1} PAIRING_PAIR_WITH_GENERATOR_X_SLOT) /\
+      pairing_pair_with_generator{2}.`2 = W256.to_uint (load Primops.memory{1} PAIRING_PAIR_WITH_GENERATOR_Y_SLOT) /\ 
+      pairing_buffer_point{2}.`1 = W256.to_uint (load Primops.memory{1} PAIRING_BUFFER_POINT_X_SLOT) /\
+      pairing_buffer_point{2}.`2 = W256.to_uint (load Primops.memory{1} PAIRING_BUFFER_POINT_Y_SLOT) /\
+      opening_proof_at_z{2}.`1 = W256.to_uint (load Primops.memory{1} PROOF_OPENING_PROOF_AT_Z_X_SLOT) /\
+      opening_proof_at_z{2}.`2 = W256.to_uint (load Primops.memory{1} PROOF_OPENING_PROOF_AT_Z_Y_SLOT) /\
+      opening_proof_at_z_omega{2}.`1 = W256.to_uint (load Primops.memory{1} PROOF_OPENING_PROOF_AT_Z_OMEGA_X_SLOT) /\
+      opening_proof_at_z_omega{2}.`2 = W256.to_uint (load Primops.memory{1} PROOF_OPENING_PROOF_AT_Z_OMEGA_Y_SLOT) /\
+      vk_recursive_flag{2} = bool_of_uint256 (load Primops.memory{1} VK_RECURSIVE_FLAG_SLOT) /\
+      recursive_part_p1{2}.`1 = W256.to_uint (load Primops.memory{1} PROOF_RECURSIVE_PART_P1_X_SLOT) /\
+      recursive_part_p1{2}.`2 = W256.to_uint (load Primops.memory{1} PROOF_RECURSIVE_PART_P1_Y_SLOT) /\
+      recursive_part_p2{2}.`1 = W256.to_uint (load Primops.memory{1} PROOF_RECURSIVE_PART_P2_X_SLOT) /\
+      recursive_part_p2{2}.`2 = W256.to_uint (load Primops.memory{1} PROOF_RECURSIVE_PART_P2_Y_SLOT) /\
+      0 <= pairing_pair_with_generator{2}.`1 < FieldQ.p /\
+      0 <= pairing_pair_with_generator{2}.`2 < FieldQ.p /\
+      0 <= pairing_buffer_point{2}.`1 < FieldQ.p /\
+      0 <= pairing_buffer_point{2}.`2 < FieldQ.p /\
+      0 <= opening_proof_at_z{2}.`1 < FieldQ.p /\
+      0 <= opening_proof_at_z{2}.`2 < FieldQ.p /\
+      0 <= opening_proof_at_z_omega{2}.`1 < FieldQ.p /\
+      0 <= opening_proof_at_z_omega{2}.`2 < FieldQ.p /\
+      0 <= u{2} < FieldR.p /\
+      0 <= z{2} < FieldR.p /\ (
+        vk_recursive_flag{2} => (
+          0 <= recursive_part_p1{2}.`1 < FieldQ.p /\
+          0 <= recursive_part_p1{2}.`2 < FieldQ.p /\
+          0 <= recursive_part_p2{2}.`1 < FieldQ.p /\
+          0 <= recursive_part_p2{2}.`2 < FieldQ.p
+        )
+      ) ==>
+      Primops.reverted{1} = !res{2}
+    ].
+    proof.
+      proc.
+      simplify.
+      
+      seq 5 6: (
+        (Primops.reverted{1} /\ failed{2}) \/ (
+          !Primops.reverted{1} /\ !failed{2} /\
+          u{2} = W256.to_uint (load Primops.memory{1} STATE_U_SLOT) /\
+          z{2} = W256.to_uint (load Primops.memory{1} STATE_Z_SLOT) /\
+           pairing_pair_with_generator{2}.`1 = W256.to_uint (load Primops.memory{1} PAIRING_PAIR_WITH_GENERATOR_X_SLOT) /\
+          pairing_pair_with_generator{2}.`2 = W256.to_uint (load Primops.memory{1} PAIRING_PAIR_WITH_GENERATOR_Y_SLOT) /\ 
+          pairing_buffer_point{2}.`1 = W256.to_uint (load Primops.memory{1} PAIRING_BUFFER_POINT_X_SLOT) /\
+          pairing_buffer_point{2}.`2 = W256.to_uint (load Primops.memory{1} PAIRING_BUFFER_POINT_Y_SLOT) /\
+          opening_proof_at_z{2}.`1 = W256.to_uint (load Primops.memory{1} PROOF_OPENING_PROOF_AT_Z_X_SLOT) /\
+          opening_proof_at_z{2}.`2 = W256.to_uint (load Primops.memory{1} PROOF_OPENING_PROOF_AT_Z_Y_SLOT) /\
+          opening_proof_at_z_omega{2}.`1 = W256.to_uint (load Primops.memory{1} PROOF_OPENING_PROOF_AT_Z_OMEGA_X_SLOT) /\
+          opening_proof_at_z_omega{2}.`2 = W256.to_uint (load Primops.memory{1} PROOF_OPENING_PROOF_AT_Z_OMEGA_Y_SLOT) /\
+          vk_recursive_flag{2} = bool_of_uint256 (load Primops.memory{1} VK_RECURSIVE_FLAG_SLOT) /\
+          recursive_part_p1{2}.`1 = W256.to_uint (load Primops.memory{1} PROOF_RECURSIVE_PART_P1_X_SLOT) /\
+          recursive_part_p1{2}.`2 = W256.to_uint (load Primops.memory{1} PROOF_RECURSIVE_PART_P1_Y_SLOT) /\
+          recursive_part_p2{2}.`1 = W256.to_uint (load Primops.memory{1} PROOF_RECURSIVE_PART_P2_X_SLOT) /\
+          recursive_part_p2{2}.`2 = W256.to_uint (load Primops.memory{1} PROOF_RECURSIVE_PART_P2_Y_SLOT) /\
+          0 <= pairing_pair_with_generator{2}.`1 < FieldQ.p /\
+          0 <= pairing_pair_with_generator{2}.`2 < FieldQ.p /\
+          0 <= pairing_buffer_point{2}.`1 < FieldQ.p /\
+          0 <= pairing_buffer_point{2}.`2 < FieldQ.p /\
+          0 <= opening_proof_at_z{2}.`1 < FieldQ.p /\
+          0 <= opening_proof_at_z{2}.`2 < FieldQ.p /\
+          0 <= opening_proof_at_z_omega{2}.`1 < FieldQ.p /\
+          0 <= opening_proof_at_z_omega{2}.`2 < FieldQ.p /\
+          0 <= u{2} < FieldR.p /\
+          0 <= z{2} < FieldR.p /\
+          u{2} = W256.to_uint u{1} /\
+          z{2} = W256.to_uint z{1} /\
+          zOmega{2} = W256.to_uint zOmega{1} /\ (
+            vk_recursive_flag{2} => (
+              0 <= recursive_part_p1{2}.`1 < FieldQ.p /\
+              0 <= recursive_part_p1{2}.`2 < FieldQ.p /\
+              0 <= recursive_part_p2{2}.`1 < FieldQ.p /\
+              0 <= recursive_part_p2{2}.`2 < FieldQ.p
+            )
+          )
+        )
+      ).
+      inline Primops.mload. sp. wp.
+      exists* Primops.memory{1}, pairing_pair_with_generator{2}, pairing_buffer_point{2}.
+      elim*=> memory_l pairing_pair_with_generator_r pairing_buffer_point_r.
+      call (pointSubAssign_low_equiv_mid_fixed memory_l PAIRING_PAIR_WITH_GENERATOR_X_SLOT PAIRING_BUFFER_POINT_X_SLOT pairing_pair_with_generator_r pairing_buffer_point_r).
+      skip.
+      progress.
+      by rewrite /PAIRING_PAIR_WITH_GENERATOR_X_SLOT W256.of_intN'; progress.
+      by rewrite /PAIRING_PAIR_WITH_GENERATOR_X_SLOT W256.of_intN'; progress.
+      by rewrite H0; reflexivity.
+      by rewrite H1; reflexivity.
+      by rewrite H2; reflexivity.
+      by rewrite H3; reflexivity.
+      case H50.
+        by progress; left; progress.
+        progress.
+          by rewrite /pointSubAssign_memory_footprint /STATE_U_SLOT /PAIRING_PAIR_WITH_GENERATOR_X_SLOT;
+          simplify;
+          do 6! ((rewrite load_store_diff; first by progress); first by progress);
+          reflexivity.
+          by rewrite /pointSubAssign_memory_footprint /STATE_Z_SLOT /PAIRING_PAIR_WITH_GENERATOR_X_SLOT;
+          simplify;
+          do 6! ((rewrite load_store_diff; first by progress); first by progress);
+          reflexivity.
+          by rewrite /pointSubAssign_memory_footprint /PAIRING_PAIR_WITH_GENERATOR_X_SLOT;
+          simplify;
+          rewrite load_store_diff; [
+            progress |
+            progress |
+            rewrite load_store_same W256.of_uintK pmod_small; progress;
+            rewrite (int_lt_lt_trans _ Constants.Q); [assumption | rewrite /Constants.Q; progress];
+            reflexivity
+          ].
+          by rewrite /pointSubAssign_memory_footprint /PAIRING_PAIR_WITH_GENERATOR_X_SLOT /PAIRING_PAIR_WITH_GENERATOR_Y_SLOT;
+          simplify;
+          rewrite load_store_same W256.of_uintK pmod_small; progress;
+          rewrite (int_lt_lt_trans _ Constants.Q); [assumption | rewrite /Constants.Q; progress];
+          reflexivity.
+          by rewrite /pointSubAssign_memory_footprint /PAIRING_BUFFER_POINT_X_SLOT /PAIRING_PAIR_WITH_GENERATOR_X_SLOT;
+          simplify;
+          do 6! ((rewrite load_store_diff; first by progress); first by progress);
+          assumption.
+          by rewrite /pointSubAssign_memory_footprint /PAIRING_BUFFER_POINT_Y_SLOT /PAIRING_PAIR_WITH_GENERATOR_X_SLOT;
+          simplify;
+          do 6! ((rewrite load_store_diff; first by progress); first by progress);
+          assumption.
+          by rewrite /pointSubAssign_memory_footprint /PROOF_OPENING_PROOF_AT_Z_X_SLOT /PAIRING_PAIR_WITH_GENERATOR_X_SLOT;
+          simplify;
+          do 6! ((rewrite load_store_diff; first by progress); first by progress);
+          assumption.
+          by rewrite /pointSubAssign_memory_footprint /PROOF_OPENING_PROOF_AT_Z_Y_SLOT /PAIRING_PAIR_WITH_GENERATOR_X_SLOT;
+          simplify;
+          do 6! ((rewrite load_store_diff; first by progress); first by progress);
+          assumption.
+          by rewrite /pointSubAssign_memory_footprint /PROOF_OPENING_PROOF_AT_Z_OMEGA_X_SLOT /PAIRING_PAIR_WITH_GENERATOR_X_SLOT;
+          simplify;
+          do 6! ((rewrite load_store_diff; first by progress); first by progress);
+          assumption.
+          by rewrite /pointSubAssign_memory_footprint /PROOF_OPENING_PROOF_AT_Z_OMEGA_Y_SLOT /PAIRING_PAIR_WITH_GENERATOR_X_SLOT;
+          simplify;
+          do 6! ((rewrite load_store_diff; first by progress); first by progress);
+          assumption.
+          by rewrite /pointSubAssign_memory_footprint /VK_RECURSIVE_FLAG_SLOT /PAIRING_PAIR_WITH_GENERATOR_X_SLOT;
+          simplify;
+          do 6! ((rewrite load_store_diff; first by progress); first by progress);
+          assumption.
+          by rewrite /pointSubAssign_memory_footprint /PROOF_RECURSIVE_PART_P1_X_SLOT /PAIRING_PAIR_WITH_GENERATOR_X_SLOT;
+          simplify;
+          do 6! ((rewrite load_store_diff; first by progress); first by progress);
+          assumption.
+          by rewrite /pointSubAssign_memory_footprint /PROOF_RECURSIVE_PART_P1_Y_SLOT /PAIRING_PAIR_WITH_GENERATOR_X_SLOT;
+          simplify;
+          do 6! ((rewrite load_store_diff; first by progress); first by progress);
+          assumption.
+          by rewrite /pointSubAssign_memory_footprint /PROOF_RECURSIVE_PART_P2_X_SLOT /PAIRING_PAIR_WITH_GENERATOR_X_SLOT;
+          simplify;
+          do 6! ((rewrite load_store_diff; first by progress); first by progress);
+          assumption.
+          by rewrite /pointSubAssign_memory_footprint /PROOF_RECURSIVE_PART_P2_Y_SLOT /PAIRING_PAIR_WITH_GENERATOR_X_SLOT;
+          simplify;
+          do 6! ((rewrite load_store_diff; first by progress); first by progress);
+          assumption.
+          by rewrite -Constants.q_eq_fieldq_p; assumption.
+          by rewrite -Constants.q_eq_fieldq_p; assumption.
+          rewrite /mulmod. simplify. rewrite -Constants.R_int /Constants.R W256.of_uintK (pmod_small _ W256.modulus).
+          progress. exact modz_ge0.
+          apply (int_lt_lt_trans _ Constants.R). rewrite /Constants.R. exact ltz_pmod. rewrite /Constants.R; progress.
+          rewrite Constants.OMEGA_int. reflexivity.
+
+          seq 1 3: #pre.
+          exists* Primops.reverted{1}. elim*=>reverted.
+          case reverted.    
+          call{1} pointMulAndAddIntoDest_low_pspec_revert.
+          inline*. wp. skip. progress.
+          left. progress. left. case H. by progress. by progress.
+
+          wp.
+          exists* opening_proof_at_z{2}, pairing_pair_with_generator{2}, z{2}, Primops.memory{1}.
+          elim*=> opening_proof_at_z_r pairing_pair_with_generator_r z_r memory_l.
+          call (pointMulAndAddIntoDest_low_equiv_mid opening_proof_at_z_r.`1 opening_proof_at_z_r.`2 pairing_pair_with_generator_r.`1 pairing_pair_with_generator_r.`2 z_r PROOF_OPENING_PROOF_AT_Z_X_SLOT PAIRING_PAIR_WITH_GENERATOR_X_SLOT memory_l).
+          skip. progress.
+          by case H; progress.
+          by case H; progress.
+          by case H; progress.
+          by case H; progress.
+          by case H; progress.
+          by case H; [
+            progress |
+            progress;
+            apply (int_lt_lt_trans _ FieldR.p); [
+              assumption |
+              rewrite -Constants.r_eq_fieldr_p /Constants.R; progress
+            ]
+          ].
+          by case H; progress.
+          by case H; progress.
+          by case H; progress.
+          by case H; progress.
+          by rewrite /PAIRING_PAIR_WITH_GENERATOR_X_SLOT W256.of_intN'; progress.
+          by rewrite /PROOF_OPENING_PROOF_AT_Z_X_SLOT; simplify; rewrite W256.of_intN'; progress.
+          by rewrite /PAIRING_PAIR_WITH_GENERATOR_X_SLOT W256.of_intN'; progress.
+          by rewrite /PAIRING_PAIR_WITH_GENERATOR_X_SLOT; simplify; rewrite W256.of_intN'; progress.
+          by case H; [progress| progress; rewrite H6; progress].
+          by case H; [progress| progress; rewrite H7; progress].
+          by case H; [progress| progress; rewrite H2; progress].
+          by case H; [progress| progress; rewrite H3; progress].
+          by case H; [progress| progress; apply uint256_eq_of_eq; rewrite H35; reflexivity].
+          case H24. progress. case H25. progress. right.
+          progress.
+          by case H; progress.
+          by case H; [
+            progress |
+            progress;
+            rewrite /STATE_U_SLOT /PAIRING_PAIR_WITH_GENERATOR_X_SLOT;
+            do 6! ((rewrite load_store_diff; first by progress); first by progress);
+            reflexivity
+          ].
+          by case H; [
+            progress |
+            progress;
+            rewrite /STATE_Z_SLOT /PAIRING_PAIR_WITH_GENERATOR_X_SLOT;
+            do 6! ((rewrite load_store_diff; first by progress); first by progress);
+            reflexivity
+          ].
+          by rewrite /PAIRING_PAIR_WITH_GENERATOR_X_SLOT load_store_diff; [
+            progress |
+            progress |
+            rewrite load_store_same W256.of_uintK pmod_small; [
+              progress; [
+                exact FieldQ.ge0_asint |
+                apply (int_lt_lt_trans _ FieldQ.p); [
+                  exact FieldQ.gtp_asint|
+                  rewrite -Constants.q_eq_fieldq_p /Constants.Q; progress
+                ]
+              ] |
+              rewrite /F_to_int_point; progress
+            ]
+          ].
+          by rewrite load_store_same W256.of_uintK pmod_small; [
+            progress; [
+              exact FieldQ.ge0_asint |
+              apply (int_lt_lt_trans _ FieldQ.p); [
+                exact FieldQ.gtp_asint|
+                rewrite -Constants.q_eq_fieldq_p /Constants.Q; progress
+              ]
+            ] |
+            rewrite /F_to_int_point; progress
+          ].
+          by case H; [ progress | progress; rewrite /PAIRING_BUFFER_POINT_X_SLOT /PAIRING_PAIR_WITH_GENERATOR_X_SLOT;
+          simplify;
+          do 6! ((rewrite load_store_diff; first by progress); first by progress);
+          assumption].
+          by case H; [ progress | progress; rewrite /PAIRING_BUFFER_POINT_Y_SLOT /PAIRING_PAIR_WITH_GENERATOR_X_SLOT;
+          simplify;
+          do 6! ((rewrite load_store_diff; first by progress); first by progress);
+          assumption].
+          by case H; [ progress | progress; rewrite /PROOF_OPENING_PROOF_AT_Z_X_SLOT /PAIRING_PAIR_WITH_GENERATOR_X_SLOT;
+          simplify;
+          do 6! ((rewrite load_store_diff; first by progress); first by progress);
+          assumption].
+          by case H; [ progress | progress; rewrite /PROOF_OPENING_PROOF_AT_Z_Y_SLOT /PAIRING_PAIR_WITH_GENERATOR_X_SLOT;
+          simplify;
+          do 6! ((rewrite load_store_diff; first by progress); first by progress);
+          assumption].
+          by case H; [ progress | progress; rewrite /PROOF_OPENING_PROOF_AT_Z_OMEGA_X_SLOT /PAIRING_PAIR_WITH_GENERATOR_X_SLOT;
+          simplify;
+          do 6! ((rewrite load_store_diff; first by progress); first by progress);
+          assumption].
+          by case H; [ progress | progress; rewrite /PROOF_OPENING_PROOF_AT_Z_OMEGA_Y_SLOT /PAIRING_PAIR_WITH_GENERATOR_X_SLOT;
+          simplify;
+          do 6! ((rewrite load_store_diff; first by progress); first by progress);
+          assumption].
+          by case H; [ progress | progress; rewrite /VK_RECURSIVE_FLAG_SLOT /PAIRING_PAIR_WITH_GENERATOR_X_SLOT;
+          simplify;
+          do 6! ((rewrite load_store_diff; first by progress); first by progress);
+          assumption].
+          by case H; [ progress | progress; rewrite /PROOF_RECURSIVE_PART_P1_X_SLOT /PAIRING_PAIR_WITH_GENERATOR_X_SLOT;
+          simplify;
+          do 6! ((rewrite load_store_diff; first by progress); first by progress);
+          assumption].
+          by case H; [ progress | progress; rewrite /PROOF_RECURSIVE_PART_P1_Y_SLOT /PAIRING_PAIR_WITH_GENERATOR_X_SLOT;
+          simplify;
+          do 6! ((rewrite load_store_diff; first by progress); first by progress);
+          assumption].
+          by case H; [ progress | progress; rewrite /PROOF_RECURSIVE_PART_P2_X_SLOT /PAIRING_PAIR_WITH_GENERATOR_X_SLOT;
+          simplify;
+          do 6! ((rewrite load_store_diff; first by progress); first by progress);
+          assumption].
+          by case H; [ progress | progress; rewrite /PROOF_RECURSIVE_PART_P2_Y_SLOT /PAIRING_PAIR_WITH_GENERATOR_X_SLOT;
+          simplify;
+          do 6! ((rewrite load_store_diff; first by progress); first by progress);
+          assumption].
+          exact F_to_int_point_1_ge_zero.
+          exact F_to_int_point_1_lt_p.
+          exact F_to_int_point_2_ge_zero.
+          exact F_to_int_point_2_lt_p.
+          by case H; progress.
+          by case H; progress.
+          by case H; progress.
+          by case H; progress.
+          by case H; progress.
+          by case H; progress.
+          by case H; progress.
+          by case H; progress.
+          by case H; progress.
+          by case H; progress.
+          by case H; progress.
+          by case H; progress.
+          by case H; progress.
+          by case H; progress.
+          case H. by progress. smt ().
+          case H. by progress. smt ().
+          case H. by progress. smt ().
+          case H. by progress. smt ().
+          case H. by progress. smt ().
+          case H. by progress. smt ().
+          case H. by progress. smt ().
+          case H. by progress. smt ().
+          by progress; left; assumption.
+          by progress; left; assumption.
+
+          seq 1 3: #pre.
+          exists* Primops.reverted{1}. elim*=>reverted.
+          case reverted.    
+          call{1} pointMulAndAddIntoDest_low_pspec_revert.
+          inline*. wp. skip. progress.
+          left. progress. left. case H. by progress. by progress.
+
+          wp.
+          exists* opening_proof_at_z_omega{2}, pairing_pair_with_generator{2}, zOmega{2}, u{2}, Primops.memory{1}.
+          elim*=> opening_proof_at_z_omega_r pairing_pair_with_generator_r zOmega_r u_r memory_l.
+          call (pointMulAndAddIntoDest_low_equiv_mid opening_proof_at_z_omega_r.`1 opening_proof_at_z_omega_r.`2 pairing_pair_with_generator_r.`1 pairing_pair_with_generator_r.`2 ((zOmega_r * u_r) %% Constants.R) PROOF_OPENING_PROOF_AT_Z_OMEGA_X_SLOT PAIRING_PAIR_WITH_GENERATOR_X_SLOT memory_l).
+          skip. progress.
+          case H; progress.
+          by case H; progress.
+          by case H; progress.
+          by case H; progress.
+          by rewrite /Constants.R; exact modz_ge0.
+          by apply (int_lt_lt_trans _ Constants.R); [
+            apply ltz_pmod; rewrite /Constants.R; progress |
+            rewrite /Constants.R; progress
+          ].
+          by case H; progress.
+          by case H; progress.
+          by case H; progress.
+          by case H; progress.
+          by rewrite /PROOF_OPENING_PROOF_AT_Z_OMEGA_X_SLOT W256.of_intN'; progress.
+          by rewrite /PROOF_OPENING_PROOF_AT_Z_OMEGA_X_SLOT; simplify; rewrite W256.of_intN'; progress.
+          by rewrite /PAIRING_PAIR_WITH_GENERATOR_X_SLOT W256.of_intN'; progress.
+          by rewrite /PAIRING_PAIR_WITH_GENERATOR_X_SLOT; simplify; rewrite W256.of_intN'; progress.
+          by case H; [progress| progress; rewrite H8; progress].
+          by case H; [progress| progress; rewrite H9; progress].
+          by case H; [progress| progress; rewrite H2; progress].
+          by case H; [progress| progress; rewrite H3; progress].
+          by case H; [
+            progress|
+            progress; rewrite /mulmod -Constants.R_int; simplify; rewrite H34; reflexivity
+          ].
+          case H25. progress. case H26. progress. right.
+          progress.
+          by case H; progress.
+          by case H; [
+            progress |
+            progress;
+            rewrite /STATE_U_SLOT /PAIRING_PAIR_WITH_GENERATOR_X_SLOT;
+            do 6! ((rewrite load_store_diff; first by progress); first by progress);
+            reflexivity
+          ].
+          by case H; [
+            progress |
+            progress;
+            rewrite /STATE_Z_SLOT /PAIRING_PAIR_WITH_GENERATOR_X_SLOT;
+            do 6! ((rewrite load_store_diff; first by progress); first by progress);
+            reflexivity
+          ].
+          by rewrite /PAIRING_PAIR_WITH_GENERATOR_X_SLOT load_store_diff; [
+            progress |
+            progress |
+            rewrite load_store_same W256.of_uintK pmod_small; [
+              progress; [
+                exact FieldQ.ge0_asint |
+                apply (int_lt_lt_trans _ FieldQ.p); [
+                  exact FieldQ.gtp_asint|
+                  rewrite -Constants.q_eq_fieldq_p /Constants.Q; progress
+                ]
+              ] |
+              rewrite /F_to_int_point; progress
+            ]
+          ].
+          by rewrite load_store_same W256.of_uintK pmod_small; [
+            progress; [
+              exact FieldQ.ge0_asint |
+              apply (int_lt_lt_trans _ FieldQ.p); [
+                exact FieldQ.gtp_asint|
+                rewrite -Constants.q_eq_fieldq_p /Constants.Q; progress
+              ]
+            ] |
+            rewrite /F_to_int_point; progress
+          ].
+          by case H; [ progress | progress; rewrite /PAIRING_BUFFER_POINT_X_SLOT /PAIRING_PAIR_WITH_GENERATOR_X_SLOT;
+          simplify;
+          do 6! ((rewrite load_store_diff; first by progress); first by progress);
+          assumption].
+          by case H; [ progress | progress; rewrite /PAIRING_BUFFER_POINT_Y_SLOT /PAIRING_PAIR_WITH_GENERATOR_X_SLOT;
+          simplify;
+          do 6! ((rewrite load_store_diff; first by progress); first by progress);
+          assumption].
+          by case H; [ progress | progress; rewrite /PROOF_OPENING_PROOF_AT_Z_X_SLOT /PAIRING_PAIR_WITH_GENERATOR_X_SLOT;
+          simplify;
+          do 6! ((rewrite load_store_diff; first by progress); first by progress);
+          assumption].
+          by case H; [ progress | progress; rewrite /PROOF_OPENING_PROOF_AT_Z_Y_SLOT /PAIRING_PAIR_WITH_GENERATOR_X_SLOT;
+          simplify;
+          do 6! ((rewrite load_store_diff; first by progress); first by progress);
+          assumption].
+          by case H; [ progress | progress; rewrite /PROOF_OPENING_PROOF_AT_Z_OMEGA_X_SLOT /PAIRING_PAIR_WITH_GENERATOR_X_SLOT;
+          simplify;
+          do 6! ((rewrite load_store_diff; first by progress); first by progress);
+          assumption].
+          by case H; [ progress | progress; rewrite /PROOF_OPENING_PROOF_AT_Z_OMEGA_Y_SLOT /PAIRING_PAIR_WITH_GENERATOR_X_SLOT;
+          simplify;
+          do 6! ((rewrite load_store_diff; first by progress); first by progress);
+          assumption].
+          by case H; [ progress | progress; rewrite /VK_RECURSIVE_FLAG_SLOT /PAIRING_PAIR_WITH_GENERATOR_X_SLOT;
+          simplify;
+          do 6! ((rewrite load_store_diff; first by progress); first by progress);
+          assumption].
+          by case H; [ progress | progress; rewrite /PROOF_RECURSIVE_PART_P1_X_SLOT /PAIRING_PAIR_WITH_GENERATOR_X_SLOT;
+          simplify;
+          do 6! ((rewrite load_store_diff; first by progress); first by progress);
+          assumption].
+          by case H; [ progress | progress; rewrite /PROOF_RECURSIVE_PART_P1_Y_SLOT /PAIRING_PAIR_WITH_GENERATOR_X_SLOT;
+          simplify;
+          do 6! ((rewrite load_store_diff; first by progress); first by progress);
+          assumption].
+          by case H; [ progress | progress; rewrite /PROOF_RECURSIVE_PART_P2_X_SLOT /PAIRING_PAIR_WITH_GENERATOR_X_SLOT;
+          simplify;
+          do 6! ((rewrite load_store_diff; first by progress); first by progress);
+          assumption].
+          by case H; [ progress | progress; rewrite /PROOF_RECURSIVE_PART_P2_Y_SLOT /PAIRING_PAIR_WITH_GENERATOR_X_SLOT;
+          simplify;
+          do 6! ((rewrite load_store_diff; first by progress); first by progress);
+          assumption].
+          exact F_to_int_point_1_ge_zero.
+          exact F_to_int_point_1_lt_p.
+          exact F_to_int_point_2_ge_zero.
+          exact F_to_int_point_2_lt_p.
+          by case H; progress.
+          by case H; progress.
+          by case H; progress.
+          by case H; progress.
+          by case H; progress.
+          by case H; progress.
+          by case H; progress.
+          by case H; progress.
+          by case H; progress.
+          by case H; progress.
+          by case H; progress.
+          by case H; progress.
+          by case H; progress.
+          by case H; progress.
+          by case H; progress.
+          case H. by progress. smt ().
+          case H. by progress. smt ().
+          case H. by progress. smt ().
+          case H. by progress. smt ().
+          case H. by progress. smt ().
+          case H. by progress. smt ().
+          case H. by progress. smt ().
+          case H. by progress. smt ().
+          by progress; left; assumption.
+          by progress; left; assumption.
+
+          seq 5 3: (
+            (Primops.reverted{1} /\ failed{2}) \/ (
+              !Primops.reverted{1} /\ !failed{2} /\
+              u{2} = W256.to_uint (load Primops.memory{1} STATE_U_SLOT) /\
+              z{2} = W256.to_uint (load Primops.memory{1} STATE_Z_SLOT) /\
+              pairing_pair_with_generator{2}.`1 = W256.to_uint (load Primops.memory{1} PAIRING_PAIR_WITH_GENERATOR_X_SLOT) /\
+              pairing_pair_with_generator{2}.`2 = W256.to_uint (load Primops.memory{1} PAIRING_PAIR_WITH_GENERATOR_Y_SLOT) /\ 
+              pairing_buffer_point{2}.`1 = W256.to_uint (load Primops.memory{1} PAIRING_BUFFER_POINT_X_SLOT) /\
+              pairing_buffer_point{2}.`2 = W256.to_uint (load Primops.memory{1} PAIRING_BUFFER_POINT_Y_SLOT) /\
+              pairing_pair_with_x{2}.`1 = W256.to_uint (load Primops.memory{1} PAIRING_PAIR_WITH_X_X_SLOT) /\
+              pairing_pair_with_x{2}.`2 = W256.to_uint (load Primops.memory{1} PAIRING_PAIR_WITH_X_Y_SLOT) /\
+              opening_proof_at_z{2}.`1 = W256.to_uint (load Primops.memory{1} PROOF_OPENING_PROOF_AT_Z_X_SLOT) /\
+              opening_proof_at_z{2}.`2 = W256.to_uint (load Primops.memory{1} PROOF_OPENING_PROOF_AT_Z_Y_SLOT) /\
+              opening_proof_at_z_omega{2}.`1 = W256.to_uint (load Primops.memory{1} PROOF_OPENING_PROOF_AT_Z_OMEGA_X_SLOT) /\
+              opening_proof_at_z_omega{2}.`2 = W256.to_uint (load Primops.memory{1} PROOF_OPENING_PROOF_AT_Z_OMEGA_Y_SLOT) /\
+              vk_recursive_flag{2} = bool_of_uint256 (load Primops.memory{1} VK_RECURSIVE_FLAG_SLOT) /\
+              recursive_part_p1{2}.`1 = W256.to_uint (load Primops.memory{1} PROOF_RECURSIVE_PART_P1_X_SLOT) /\
+              recursive_part_p1{2}.`2 = W256.to_uint (load Primops.memory{1} PROOF_RECURSIVE_PART_P1_Y_SLOT) /\
+              recursive_part_p2{2}.`1 = W256.to_uint (load Primops.memory{1} PROOF_RECURSIVE_PART_P2_X_SLOT) /\
+              recursive_part_p2{2}.`2 = W256.to_uint (load Primops.memory{1} PROOF_RECURSIVE_PART_P2_Y_SLOT) /\
+              0 <= pairing_pair_with_generator{2}.`1 < FieldQ.p /\
+              0 <= pairing_pair_with_generator{2}.`2 < FieldQ.p /\
+              0 <= pairing_buffer_point{2}.`1 < FieldQ.p /\
+              0 <= pairing_buffer_point{2}.`2 < FieldQ.p /\
+              0 <= pairing_pair_with_x{2}.`1 < FieldQ.p /\
+              0 <= pairing_pair_with_x{2}.`2 < FieldQ.p /\
+              0 <= opening_proof_at_z{2}.`1 < FieldQ.p /\
+              0 <= opening_proof_at_z{2}.`2 < FieldQ.p /\
+              0 <= opening_proof_at_z_omega{2}.`1 < FieldQ.p /\
+              0 <= opening_proof_at_z_omega{2}.`2 < FieldQ.p /\
+              0 <= u{2} < FieldR.p /\
+              0 <= z{2} < FieldR.p /\
+              u{2} = W256.to_uint u{1} /\
+              z{2} = W256.to_uint z{1} /\
+              zOmega{2} = W256.to_uint zOmega{1} /\ (
+                vk_recursive_flag{2} => (
+                  0 <= recursive_part_p1{2}.`1 < FieldQ.p /\
+                  0 <= recursive_part_p1{2}.`2 < FieldQ.p /\
+                  0 <= recursive_part_p2{2}.`1 < FieldQ.p /\
+                  0 <= recursive_part_p2{2}.`2 < FieldQ.p
+                )
+              )
+            )  
+          ).
+          inline Primops.mload Primops.mstore.
+          sp. wp.
+          exists* Primops.reverted{1}. elim*=> reverted.
+          case reverted. progress.
+          call{1} pointMulAndAddIntoDest_low_pspec_revert.
+          inline*. wp. skip. progress.
+          left. progress. left. by progress.
+
+          progress.
+          exists* opening_proof_at_z_omega{2}, opening_proof_at_z{2}, u{2}, Primops.memory{1}.
+          elim*=> opening_proof_at_z_omega_r opening_proof_at_z_r u_r memory_l.
+          call (pointMulAndAddIntoDest_low_equiv_mid opening_proof_at_z_omega_r.`1 opening_proof_at_z_omega_r.`2 opening_proof_at_z_r.`1 opening_proof_at_z_r.`2 u_r PROOF_OPENING_PROOF_AT_Z_OMEGA_X_SLOT PAIRING_PAIR_WITH_X_X_SLOT memory_l).
+          skip. progress.
+          exact to_uint_lt_mod.
+          by rewrite /PROOF_OPENING_PROOF_AT_Z_OMEGA_X_SLOT W256.of_intN'; progress.
+          by rewrite /PROOF_OPENING_PROOF_AT_Z_OMEGA_X_SLOT; simplify; rewrite W256.of_intN'; progress.
+          by rewrite /PAIRING_PAIR_WITH_X_X_SLOT W256.of_intN'; progress.
+          by rewrite /PAIRING_PAIR_WITH_X_X_SLOT; simplify; rewrite W256.of_intN'; progress.
+          by rewrite load_store_diff; [
+            rewrite /PROOF_OPENING_PROOF_AT_Z_OMEGA_X_SLOT /PAIRING_PAIR_WITH_X_Y_SLOT; progress |
+            rewrite /PROOF_OPENING_PROOF_AT_Z_OMEGA_X_SLOT /PAIRING_PAIR_WITH_X_Y_SLOT; progress |
+            rewrite load_store_diff; [
+              rewrite /PROOF_OPENING_PROOF_AT_Z_OMEGA_X_SLOT /PAIRING_PAIR_WITH_X_X_SLOT; progress |
+              rewrite /PROOF_OPENING_PROOF_AT_Z_OMEGA_X_SLOT /PAIRING_PAIR_WITH_X_X_SLOT; progress |
+              rewrite H7; progress
+            ]
+          ].
+          by rewrite load_store_diff; [
+            rewrite /PROOF_OPENING_PROOF_AT_Z_OMEGA_X_SLOT /PAIRING_PAIR_WITH_X_Y_SLOT; progress |
+            rewrite /PROOF_OPENING_PROOF_AT_Z_OMEGA_X_SLOT /PAIRING_PAIR_WITH_X_Y_SLOT; progress |
+            rewrite load_store_diff; [
+              rewrite /PROOF_OPENING_PROOF_AT_Z_OMEGA_X_SLOT /PAIRING_PAIR_WITH_X_X_SLOT; progress |
+              rewrite /PROOF_OPENING_PROOF_AT_Z_OMEGA_X_SLOT /PAIRING_PAIR_WITH_X_X_SLOT; progress |
+              rewrite H8; progress
+            ]
+          ].
+          by rewrite load_store_diff; [
+            rewrite /PAIRING_PAIR_WITH_X_X_SLOT /PAIRING_PAIR_WITH_X_Y_SLOT; progress |
+            rewrite /PAIRING_PAIR_WITH_X_X_SLOT /PAIRING_PAIR_WITH_X_Y_SLOT; progress |
+            rewrite load_store_same H5; progress
+          ].
+          by rewrite load_store_same /PAIRING_PAIR_WITH_X_X_SLOT /PROOF_OPENING_PROOF_AT_Z_Y_SLOT H6 load_store_diff; progress.
+          by apply uint256_eq_of_eq; rewrite H33; reflexivity.
+          case H58. progress. case H59. progress. right. progress.
+          by rewrite /STATE_U_SLOT /PAIRING_PAIR_WITH_X_X_SLOT /PROOF_OPENING_PROOF_AT_Z_Y_SLOT /PROOF_OPENING_PROOF_AT_Z_X_SLOT /PAIRING_PAIR_WITH_X_Y_SLOT;
+            do 8! ((rewrite load_store_diff; first by progress); first by progress);
+            reflexivity.
+          by rewrite /STATE_Z_SLOT /PAIRING_PAIR_WITH_X_X_SLOT /PROOF_OPENING_PROOF_AT_Z_Y_SLOT /PROOF_OPENING_PROOF_AT_Z_X_SLOT /PAIRING_PAIR_WITH_X_Y_SLOT;
+            do 8! ((rewrite load_store_diff; first by progress); first by progress);
+            reflexivity.
+          by rewrite H1 /PAIRING_PAIR_WITH_GENERATOR_X_SLOT /PAIRING_PAIR_WITH_X_X_SLOT /PROOF_OPENING_PROOF_AT_Z_Y_SLOT /PROOF_OPENING_PROOF_AT_Z_X_SLOT /PAIRING_PAIR_WITH_X_Y_SLOT;
+            do 8! ((rewrite load_store_diff; first by progress); first by progress);
+            reflexivity.
+          by rewrite H2 /PAIRING_PAIR_WITH_GENERATOR_Y_SLOT /PAIRING_PAIR_WITH_X_X_SLOT /PROOF_OPENING_PROOF_AT_Z_Y_SLOT /PROOF_OPENING_PROOF_AT_Z_X_SLOT /PAIRING_PAIR_WITH_X_Y_SLOT;
+            do 8! ((rewrite load_store_diff; first by progress); first by progress);
+            reflexivity.
+          by rewrite H3 /PAIRING_BUFFER_POINT_X_SLOT /PAIRING_PAIR_WITH_X_X_SLOT /PROOF_OPENING_PROOF_AT_Z_Y_SLOT /PROOF_OPENING_PROOF_AT_Z_X_SLOT /PAIRING_PAIR_WITH_X_Y_SLOT;
+            do 8! ((rewrite load_store_diff; first by progress); first by progress);
+            reflexivity.
+          by rewrite H4 /PAIRING_BUFFER_POINT_Y_SLOT /PAIRING_PAIR_WITH_X_X_SLOT /PROOF_OPENING_PROOF_AT_Z_Y_SLOT /PROOF_OPENING_PROOF_AT_Z_X_SLOT /PAIRING_PAIR_WITH_X_Y_SLOT;
+            do 8! ((rewrite load_store_diff; first by progress); first by progress);
+            reflexivity.
+          by rewrite /PAIRING_PAIR_WITH_X_X_SLOT load_store_diff; [
+            progress |
+            progress |
+            rewrite load_store_same /F_to_int_point W256.of_uintK pmod_small; progress; [
+              exact FieldQ.ge0_asint |
+              apply (int_lt_lt_trans _ FieldQ.p); [exact FieldQ.gtp_asint| rewrite -Constants.q_eq_fieldq_p /Constants.Q; progress]
+            ]
+          ].
+          by rewrite load_store_same /F_to_int_point W256.of_uintK pmod_small; progress; [
+            exact FieldQ.ge0_asint |
+            apply (int_lt_lt_trans _ FieldQ.p); [exact FieldQ.gtp_asint| rewrite -Constants.q_eq_fieldq_p /Constants.Q; progress]
+          ].
+          by rewrite H5 /PROOF_OPENING_PROOF_AT_Z_X_SLOT /PAIRING_PAIR_WITH_X_X_SLOT /PROOF_OPENING_PROOF_AT_Z_Y_SLOT /PROOF_OPENING_PROOF_AT_Z_X_SLOT /PAIRING_PAIR_WITH_X_Y_SLOT;
+            do 8! ((rewrite load_store_diff; first by progress); first by progress);
+            reflexivity.
+          by rewrite H6 /PROOF_OPENING_PROOF_AT_Z_Y_SLOT /PAIRING_PAIR_WITH_X_X_SLOT /PROOF_OPENING_PROOF_AT_Z_Y_SLOT /PROOF_OPENING_PROOF_AT_Z_X_SLOT /PAIRING_PAIR_WITH_X_Y_SLOT;
+            do 8! ((rewrite load_store_diff; first by progress); first by progress);
+            reflexivity.
+          by rewrite H7 /PROOF_OPENING_PROOF_AT_Z_OMEGA_X_SLOT /PAIRING_PAIR_WITH_X_X_SLOT /PROOF_OPENING_PROOF_AT_Z_Y_SLOT /PROOF_OPENING_PROOF_AT_Z_X_SLOT /PAIRING_PAIR_WITH_X_Y_SLOT;
+            do 8! ((rewrite load_store_diff; first by progress); first by progress);
+            reflexivity.
+          by rewrite H8 /PROOF_OPENING_PROOF_AT_Z_OMEGA_Y_SLOT /PAIRING_PAIR_WITH_X_X_SLOT /PROOF_OPENING_PROOF_AT_Z_Y_SLOT /PROOF_OPENING_PROOF_AT_Z_X_SLOT /PAIRING_PAIR_WITH_X_Y_SLOT;
+            do 8! ((rewrite load_store_diff; first by progress); first by progress);
+            reflexivity.
+          by rewrite /VK_RECURSIVE_FLAG_SLOT /PAIRING_PAIR_WITH_X_X_SLOT /PROOF_OPENING_PROOF_AT_Z_Y_SLOT /PROOF_OPENING_PROOF_AT_Z_X_SLOT /PAIRING_PAIR_WITH_X_Y_SLOT;
+            do 8! ((rewrite load_store_diff; first by progress); first by progress);
+            reflexivity.
+          by rewrite H9 /PROOF_RECURSIVE_PART_P1_X_SLOT /PAIRING_PAIR_WITH_X_X_SLOT /PROOF_OPENING_PROOF_AT_Z_Y_SLOT /PROOF_OPENING_PROOF_AT_Z_X_SLOT /PAIRING_PAIR_WITH_X_Y_SLOT;
+            do 8! ((rewrite load_store_diff; first by progress); first by progress);
+            reflexivity.
+          by rewrite H10 /PROOF_RECURSIVE_PART_P1_Y_SLOT /PAIRING_PAIR_WITH_X_X_SLOT /PROOF_OPENING_PROOF_AT_Z_Y_SLOT /PROOF_OPENING_PROOF_AT_Z_X_SLOT /PAIRING_PAIR_WITH_X_Y_SLOT;
+            do 8! ((rewrite load_store_diff; first by progress); first by progress);
+            reflexivity.
+          by rewrite H11 /PROOF_RECURSIVE_PART_P2_X_SLOT /PAIRING_PAIR_WITH_X_X_SLOT /PROOF_OPENING_PROOF_AT_Z_Y_SLOT /PROOF_OPENING_PROOF_AT_Z_X_SLOT /PAIRING_PAIR_WITH_X_Y_SLOT;
+            do 8! ((rewrite load_store_diff; first by progress); first by progress);
+            reflexivity.
+          by rewrite H12 /PROOF_RECURSIVE_PART_P2_Y_SLOT /PAIRING_PAIR_WITH_X_X_SLOT /PROOF_OPENING_PROOF_AT_Z_Y_SLOT /PROOF_OPENING_PROOF_AT_Z_X_SLOT /PAIRING_PAIR_WITH_X_Y_SLOT;
+            do 8! ((rewrite load_store_diff; first by progress); first by progress);
+            reflexivity.
+          exact F_to_int_point_1_ge_zero.
+          exact F_to_int_point_1_lt_p.
+          exact F_to_int_point_2_ge_zero.
+          exact F_to_int_point_2_lt_p.
+          by progress; left; progress.
+          by progress; left; progress.
+
+          seq 1 3: #pre.
+          exists* Primops.reverted{1}. elim*=> reverted.
+          case reverted.
+          inline*. wp. skip. progress. case H; by progress.
+          left. progress. case H; by progress.
+          left. progress. case H; by progress.
+
+          exists* Primops.memory{1}, pairing_pair_with_x{2}.
+          elim*=> memory_l pairing_pair_with_x_r.
+          wp.
+          call (pointNegate_low_equiv_mid memory_l PAIRING_PAIR_WITH_X_X_SLOT pairing_pair_with_x_r.`1 pairing_pair_with_x_r.`2).
+          skip. progress.
+          smt ().
+          by rewrite Constants.q_eq_fieldq_p; case H; by progress.
+          by rewrite Constants.q_eq_fieldq_p; case H; by progress.
+          case H. by progress. progress. rewrite H6. reflexivity.
+          case H. by progress. progress. rewrite H7. reflexivity.
+          case H. by progress. case H7. by progress. progress. right. progress.
+          by rewrite /STATE_U_SLOT /PAIRING_PAIR_WITH_X_X_SLOT load_store_diff; [
+            progress |
+            progress |
+            rewrite load_store_diff; [
+              progress |
+              progress |
+              reflexivity
+            ]
+          ].
+          by rewrite /STATE_Z_SLOT /PAIRING_PAIR_WITH_X_X_SLOT load_store_diff; [
+            progress |
+            progress |
+            rewrite load_store_diff; [
+              progress |
+              progress |
+              reflexivity
+            ]
+          ].
+          by rewrite /PAIRING_PAIR_WITH_GENERATOR_X_SLOT /PAIRING_PAIR_WITH_X_X_SLOT load_store_diff; [
+            progress |
+            progress |
+            rewrite load_store_diff; [
+              progress |
+              progress |
+              rewrite H13; reflexivity
+            ]
+          ].  
+          by rewrite /PAIRING_PAIR_WITH_GENERATOR_Y_SLOT /PAIRING_PAIR_WITH_X_X_SLOT load_store_diff; [
+            progress |
+            progress |
+            rewrite load_store_diff; [
+              progress |
+              progress |
+              rewrite H14; reflexivity
+            ]
+          ].
+          by rewrite /PAIRING_BUFFER_POINT_X_SLOT /PAIRING_PAIR_WITH_X_X_SLOT load_store_diff; [
+            progress |
+            progress |
+            rewrite load_store_diff; [
+              progress |
+              progress |
+              rewrite H15; reflexivity
+            ]
+          ].  
+          by rewrite /PAIRING_BUFFER_POINT_Y_SLOT /PAIRING_PAIR_WITH_X_X_SLOT load_store_diff; [
+            progress |
+            progress |
+            rewrite load_store_diff; [
+              progress |
+              progress |
+              rewrite H16; reflexivity
+            ]
+          ].
+          by rewrite /PAIRING_PAIR_WITH_X_X_SLOT load_store_diff; [
+            progress |
+            progress |
+            rewrite load_store_same W256.of_uintK pmod_small; progress;
+              apply (int_lt_lt_trans _ Constants.Q); [
+                assumption |
+                rewrite /Constants.Q; progress; reflexivity
+              ]
+          ].
+          by rewrite load_store_same W256.of_uintK pmod_small; progress;
+            apply (int_lt_lt_trans _ Constants.Q); [
+              assumption |
+              rewrite /Constants.Q; progress; reflexivity
+            ].
+          by rewrite /PROOF_OPENING_PROOF_AT_Z_X_SLOT /PAIRING_PAIR_WITH_X_X_SLOT load_store_diff; [
+            progress |
+            progress |
+            rewrite load_store_diff; [
+              progress |
+              progress |
+              rewrite H19; reflexivity
+            ]
+          ].  
+          by rewrite /PROOF_OPENING_PROOF_AT_Z_Y_SLOT /PAIRING_PAIR_WITH_X_X_SLOT load_store_diff; [
+            progress |
+            progress |
+            rewrite load_store_diff; [
+              progress |
+              progress |
+              rewrite H20; reflexivity
+            ]
+          ].
+          by rewrite /PROOF_OPENING_PROOF_AT_Z_OMEGA_X_SLOT /PAIRING_PAIR_WITH_X_X_SLOT load_store_diff; [
+            progress |
+            progress |
+            rewrite load_store_diff; [
+              progress |
+              progress |
+              rewrite H21; reflexivity
+            ]
+          ].  
+          by rewrite /PROOF_OPENING_PROOF_AT_Z_OMEGA_Y_SLOT /PAIRING_PAIR_WITH_X_X_SLOT load_store_diff; [
+            progress |
+            progress |
+            rewrite load_store_diff; [
+              progress |
+              progress |
+              rewrite H22; reflexivity
+            ]
+          ].
+          by rewrite /VK_RECURSIVE_FLAG_SLOT /PAIRING_PAIR_WITH_X_X_SLOT load_store_diff; [
+            progress |
+            progress |
+            rewrite load_store_diff; [
+              progress |
+              progress |
+              reflexivity
+            ]
+          ].
+          by rewrite /PROOF_RECURSIVE_PART_P1_X_SLOT /PAIRING_PAIR_WITH_X_X_SLOT load_store_diff; [
+            progress |
+            progress |
+            rewrite load_store_diff; [
+              progress |
+              progress |
+              rewrite H23; reflexivity
+            ]
+          ].  
+          by rewrite /PROOF_RECURSIVE_PART_P1_Y_SLOT /PAIRING_PAIR_WITH_X_X_SLOT load_store_diff; [
+            progress |
+            progress |
+            rewrite load_store_diff; [
+              progress |
+              progress |
+              rewrite H24; reflexivity
+            ]
+          ].
+          by rewrite /PROOF_RECURSIVE_PART_P2_X_SLOT /PAIRING_PAIR_WITH_X_X_SLOT load_store_diff; [
+            progress |
+            progress |
+            rewrite load_store_diff; [
+              progress |
+              progress |
+              rewrite H25; reflexivity
+            ]
+          ].  
+          by rewrite /PROOF_RECURSIVE_PART_P2_Y_SLOT /PAIRING_PAIR_WITH_X_X_SLOT load_store_diff; [
+            progress |
+            progress |
+            rewrite load_store_diff; [
+              progress |
+              progress |
+              rewrite H26; reflexivity
+            ]
+          ].
+          by rewrite -Constants.q_eq_fieldq_p; assumption.
+          by rewrite -Constants.q_eq_fieldq_p; assumption.
+
+          seq 2 1: #pre.
+          exists* Primops.reverted{1}. elim*=> reverted.
+          case reverted.
+          conseq (_: Primops.reverted{1} /\ failed{2} ==> Primops.reverted{1} /\ failed{2}).
+          progress. by case H; progress.
+          progress. left. by progress.
+          inline Primops.mload. sp.
+          case (vk_recursive_flag{2}).
+          rcondt{2} 1. by progress.
+          case (bool_of_uint256 _17{1}).
+          rcondt{1} 1. by progress.
+          call{1} pointMulAndAddIntoDest_low_pspec_revert.
+          call{1} pointMulAndAddIntoDest_low_pspec_revert.
+          inline*. wp. skip.
+          progress. left. left. assumption.
+          rcondf{1} 1. by progress.
+          inline*. wp. skip. progress. left. left. assumption.
+          rcondf{2} 1. by progress.
+          case (bool_of_uint256 _17{1}).
+          rcondt{1} 1. by progress.
+          call{1} pointMulAndAddIntoDest_low_pspec_revert.
+          call{1} pointMulAndAddIntoDest_low_pspec_revert.
+          inline*. wp. skip.
+          by progress.
+          rcondf{1} 1. by progress. skip. by progress.
+
+          case (vk_recursive_flag{2}).
+          rcondt{2} 1. by progress.
+          rcondt{1} 2. progress. inline*. wp. skip. progress; case H; by progress.
+          
+          seq 2 1: (
+            !Primops.reverted{1} /\ !failed{2} /\
+            u{2} = W256.to_uint (load Primops.memory{1} STATE_U_SLOT) /\
+            z{2} = W256.to_uint (load Primops.memory{1} STATE_Z_SLOT) /\
+            pairing_pair_with_generator{2}.`1 = W256.to_uint (load Primops.memory{1} PAIRING_PAIR_WITH_GENERATOR_X_SLOT) /\
+            pairing_pair_with_generator{2}.`2 = W256.to_uint (load Primops.memory{1} PAIRING_PAIR_WITH_GENERATOR_Y_SLOT) /\ 
+            pairing_buffer_point{2}.`1 = W256.to_uint (load Primops.memory{1} PAIRING_BUFFER_POINT_X_SLOT) /\
+            pairing_buffer_point{2}.`2 = W256.to_uint (load Primops.memory{1} PAIRING_BUFFER_POINT_Y_SLOT) /\
+            pairing_pair_with_x{2}.`1 = W256.to_uint (load Primops.memory{1} PAIRING_PAIR_WITH_X_X_SLOT) /\
+            pairing_pair_with_x{2}.`2 = W256.to_uint (load Primops.memory{1} PAIRING_PAIR_WITH_X_Y_SLOT) /\
+            opening_proof_at_z{2}.`1 = W256.to_uint (load Primops.memory{1} PROOF_OPENING_PROOF_AT_Z_X_SLOT) /\
+            opening_proof_at_z{2}.`2 = W256.to_uint (load Primops.memory{1} PROOF_OPENING_PROOF_AT_Z_Y_SLOT) /\
+            opening_proof_at_z_omega{2}.`1 = W256.to_uint (load Primops.memory{1} PROOF_OPENING_PROOF_AT_Z_OMEGA_X_SLOT) /\
+            opening_proof_at_z_omega{2}.`2 = W256.to_uint (load Primops.memory{1} PROOF_OPENING_PROOF_AT_Z_OMEGA_Y_SLOT) /\
+            vk_recursive_flag{2} = bool_of_uint256 (load Primops.memory{1} VK_RECURSIVE_FLAG_SLOT) /\
+            recursive_part_p1{2}.`1 = W256.to_uint (load Primops.memory{1} PROOF_RECURSIVE_PART_P1_X_SLOT) /\
+            recursive_part_p1{2}.`2 = W256.to_uint (load Primops.memory{1} PROOF_RECURSIVE_PART_P1_Y_SLOT) /\
+            recursive_part_p2{2}.`1 = W256.to_uint (load Primops.memory{1} PROOF_RECURSIVE_PART_P2_X_SLOT) /\
+            recursive_part_p2{2}.`2 = W256.to_uint (load Primops.memory{1} PROOF_RECURSIVE_PART_P2_Y_SLOT) /\
+            0 <= pairing_pair_with_generator{2}.`1 < FieldQ.p /\
+            0 <= pairing_pair_with_generator{2}.`2 < FieldQ.p /\
+            0 <= pairing_buffer_point{2}.`1 < FieldQ.p /\
+            0 <= pairing_buffer_point{2}.`2 < FieldQ.p /\
+            0 <= pairing_pair_with_x{2}.`1 < FieldQ.p /\
+            0 <= pairing_pair_with_x{2}.`2 < FieldQ.p /\
+            0 <= opening_proof_at_z{2}.`1 < FieldQ.p /\
+            0 <= opening_proof_at_z{2}.`2 < FieldQ.p /\
+            0 <= opening_proof_at_z_omega{2}.`1 < FieldQ.p /\
+            0 <= opening_proof_at_z_omega{2}.`2 < FieldQ.p /\
+            0 <= u{2} < FieldR.p /\
+            0 <= z{2} < FieldR.p /\
+            u{2} = W256.to_uint u{1} /\
+            z{2} = W256.to_uint z{1} /\
+            zOmega{2} = W256.to_uint zOmega{1} /\
+            0 <= recursive_part_p1{2}.`1 < FieldQ.p /\
+            0 <= recursive_part_p1{2}.`2 < FieldQ.p /\
+            0 <= recursive_part_p2{2}.`1 < FieldQ.p /\
+            0 <= recursive_part_p2{2}.`2 < FieldQ.p /\
+            uu{2} = W256.to_uint uu{1} /\
+            vk_recursive_flag{2}
+          ).
+          inline*. wp. skip. progress.
+          by case H; progress.
+          by case H; progress.
+          by case H; progress.
+          by case H; progress.
+          by case H; progress.
+          by case H; progress.
+          by case H; progress.
+          by case H; progress.
+          by case H; progress.
+          by case H; progress.
+          by case H; progress.
+          by case H; progress.
+          by case H; progress.
+          by case H; progress.
+          by case H; progress.
+          by case H; progress.
+          by case H; progress.
+          by case H; progress.
+          by case H; progress.
+          by case H; progress.
+          by case H; progress.
+          by case H; progress.
+          by case H; progress.
+          by case H; progress.
+          by case H; progress.
+          by case H; progress.
+          by case H; progress.
+          by case H; progress.
+          by case H; progress.
+          by case H; progress.
+          by case H; progress.
+          by case H; progress.
+          by case H; progress.
+          by case H; progress.
+          by case H; progress.
+          by case H; progress.
+          by case H; progress.
+          by case H; progress.
+          by case H; progress.
+          by case H; progress.
+          by case H; progress.
+          by case H; progress.
+          by case H; progress.
+          by case H; progress.
+          by case H; progress.
+          by case H; [progress | rewrite H1; progress].
+          by case H; [progress | rewrite H1; progress].
+          by case H; [progress | rewrite H1; progress].
+          by case H; [progress | rewrite H1; progress].
+          by case H; [progress | rewrite H1; progress].
+          by case H; [progress | rewrite H1; progress].
+          by case H; [progress | rewrite H1; progress].
+          by case H; [progress | rewrite H1; progress].
+          rewrite /mulmod. simplify. rewrite W256.of_uintK (pmod_small _ W256.modulus).
+          progress. apply modz_ge0. rewrite -Constants.R_int /Constants.R. by trivial.
+          apply (int_lt_lt_trans _ Constants.R). rewrite -Constants.R_int /Constants.R. exact ltz_pmod.
+          rewrite /Constants.R. by trivial.
+          rewrite -Constants.R_int. case H; progress. rewrite H41. reflexivity.
+
+          seq 1 3: (
+            #pre \/ (Primops.reverted{1} /\ failed{2})
+          ).
+          wp.
+          exists* recursive_part_p1{2}, pairing_pair_with_generator{2}, uu{2}, Primops.memory{1}.
+          elim*=> recursive_part_p1_r pairing_pair_with_generator_r uu_r memory_l.
+          call (pointMulAndAddIntoDest_low_equiv_mid recursive_part_p1_r.`1 recursive_part_p1_r.`2 pairing_pair_with_generator_r.`1 pairing_pair_with_generator_r.`2 uu_r PROOF_RECURSIVE_PART_P1_X_SLOT PAIRING_PAIR_WITH_GENERATOR_X_SLOT memory_l).
+          skip. progress.
+          exact to_uint_ge_zero. exact to_uint_lt_mod.
+          by rewrite /PROOF_RECURSIVE_PART_P1_X_SLOT W256.of_intN'; progress.
+          by rewrite /PROOF_RECURSIVE_PART_P1_X_SLOT; simplify; rewrite W256.of_intN'; progress.
+          by rewrite /PAIRING_PAIR_WITH_GENERATOR_X_SLOT W256.of_intN'; progress.
+          by rewrite /PAIRING_PAIR_WITH_GENERATOR_X_SLOT; simplify; rewrite W256.of_intN'; progress.
+          by rewrite H11; progress.
+          by rewrite H12; progress.
+          by rewrite H1; progress.
+          by rewrite H2; progress.
+          case H73. progress. case H74. progress.
+            left. progress.
+            by rewrite /STATE_U_SLOT /PAIRING_PAIR_WITH_GENERATOR_X_SLOT;
+            do 6! ((rewrite load_store_diff; first by progress); first by progress);
+            reflexivity.
+            by rewrite /STATE_Z_SLOT /PAIRING_PAIR_WITH_GENERATOR_X_SLOT;
+            do 6! ((rewrite load_store_diff; first by progress); first by progress);
+            reflexivity.
+            rewrite /PAIRING_PAIR_WITH_GENERATOR_X_SLOT load_store_diff.
+              by progress.
+              by progress.
+              rewrite load_store_same /F_to_int_point. simplify.
+              rewrite W256.of_uintK pmod_small. progress.
+                exact FieldQ.ge0_asint.
+                apply (int_lt_lt_trans _ FieldQ.p).
+                  exact FieldQ.gtp_asint. rewrite -Constants.q_eq_fieldq_p /Constants.Q. by trivial.
+                reflexivity.
+            rewrite load_store_same /F_to_int_point. simplify.
+            rewrite W256.of_uintK pmod_small. progress.
+            exact FieldQ.ge0_asint.
+            apply (int_lt_lt_trans _ FieldQ.p).
+            exact FieldQ.gtp_asint. rewrite -Constants.q_eq_fieldq_p /Constants.Q. by trivial.
+            reflexivity.
+            by rewrite /PAIRING_BUFFER_POINT_X_SLOT /PAIRING_PAIR_WITH_GENERATOR_X_SLOT;
+            do 6! ((rewrite load_store_diff; first by progress); first by progress);
+            rewrite H3; reflexivity.
+            by rewrite /PAIRING_BUFFER_POINT_Y_SLOT /PAIRING_PAIR_WITH_GENERATOR_X_SLOT;
+            do 6! ((rewrite load_store_diff; first by progress); first by progress);
+            rewrite H4; reflexivity.
+            by rewrite /PAIRING_PAIR_WITH_X_X_SLOT /PAIRING_PAIR_WITH_GENERATOR_X_SLOT;
+            do 6! ((rewrite load_store_diff; first by progress); first by progress);
+            rewrite H5; reflexivity.
+            by rewrite /PAIRING_PAIR_WITH_X_Y_SLOT /PAIRING_PAIR_WITH_GENERATOR_X_SLOT;
+            do 6! ((rewrite load_store_diff; first by progress); first by progress);
+            rewrite H6; reflexivity.
+            by rewrite /PROOF_OPENING_PROOF_AT_Z_X_SLOT /PAIRING_PAIR_WITH_GENERATOR_X_SLOT;
+            do 6! ((rewrite load_store_diff; first by progress); first by progress);
+            rewrite H7; reflexivity.
+            by rewrite /PROOF_OPENING_PROOF_AT_Z_Y_SLOT /PAIRING_PAIR_WITH_GENERATOR_X_SLOT;
+            do 6! ((rewrite load_store_diff; first by progress); first by progress);
+            rewrite H8; reflexivity.
+            by rewrite /PROOF_OPENING_PROOF_AT_Z_OMEGA_X_SLOT /PAIRING_PAIR_WITH_GENERATOR_X_SLOT;
+            do 6! ((rewrite load_store_diff; first by progress); first by progress);
+            rewrite H9; reflexivity.
+            by rewrite /PROOF_OPENING_PROOF_AT_Z_OMEGA_Y_SLOT /PAIRING_PAIR_WITH_GENERATOR_X_SLOT;
+            do 6! ((rewrite load_store_diff; first by progress); first by progress);
+            rewrite H10; reflexivity.
+            by rewrite /VK_RECURSIVE_FLAG_SLOT /PAIRING_PAIR_WITH_GENERATOR_X_SLOT;
+            do 6! ((rewrite load_store_diff; first by progress); first by progress);
+            reflexivity.
+            by rewrite /PROOF_RECURSIVE_PART_P1_X_SLOT /PAIRING_PAIR_WITH_GENERATOR_X_SLOT;
+            do 6! ((rewrite load_store_diff; first by progress); first by progress);
+            rewrite H11; reflexivity.
+            by rewrite /PROOF_RECURSIVE_PART_P1_Y_SLOT /PAIRING_PAIR_WITH_GENERATOR_X_SLOT;
+            do 6! ((rewrite load_store_diff; first by progress); first by progress);
+            rewrite H12; reflexivity.
+            by rewrite /PROOF_RECURSIVE_PART_P2_X_SLOT /PAIRING_PAIR_WITH_GENERATOR_X_SLOT;
+            do 6! ((rewrite load_store_diff; first by progress); first by progress);
+            rewrite H13; reflexivity.
+            by rewrite /PROOF_RECURSIVE_PART_P2_Y_SLOT /PAIRING_PAIR_WITH_GENERATOR_X_SLOT;
+            do 6! ((rewrite load_store_diff; first by progress); first by progress);
+            rewrite H14; reflexivity.
+            exact F_to_int_point_1_ge_zero.
+            exact F_to_int_point_1_lt_p.
+            exact F_to_int_point_2_ge_zero.
+            exact F_to_int_point_2_lt_p.
+            by progress.
+            by progress.
+
+          case (Primops.reverted{1}).
+          call{1} pointMulAndAddIntoDest_low_pspec_revert.
+          inline*. wp. skip. progress. left. progress. left. case H. by progress. by progress.
+
+          wp.
+          exists* recursive_part_p2{2}, pairing_pair_with_x{2}, uu{2}, Primops.memory{1}.
+          elim*=> recursive_part_p2_r pairing_pair_with_x_r uu_r memory_l.
+          call (pointMulAndAddIntoDest_low_equiv_mid recursive_part_p2_r.`1 recursive_part_p2_r.`2 pairing_pair_with_x_r.`1 pairing_pair_with_x_r.`2 uu_r PROOF_RECURSIVE_PART_P2_X_SLOT PAIRING_PAIR_WITH_X_X_SLOT memory_l).
+          skip. progress.
+          by case H; progress.
+          by case H; progress.
+          by case H; progress.
+          by case H; progress.
+          case H. by progress; exact to_uint_ge_zero. by progress.
+          case H. by progress; exact to_uint_lt_mod. by progress.
+          by case H; progress.
+          by case H; progress.
+          by case H; progress.
+          by case H; progress.
+          by rewrite /PROOF_RECURSIVE_PART_P2_X_SLOT W256.of_intN'; progress.
+          by rewrite /PROOF_RECURSIVE_PART_P2_X_SLOT; simplify; rewrite W256.of_intN'; progress.
+          by rewrite /PAIRING_PAIR_WITH_X_X_SLOT W256.of_intN'; progress.
+          by rewrite /PAIRING_PAIR_WITH_X_X_SLOT; simplify; rewrite W256.of_intN'; progress.
+          case H. progress. rewrite H14. by progress. by progress.
+          case H. progress. rewrite H15. by progress. by progress.
+          case H. progress. rewrite H6. by progress. by progress.
+          case H. progress. rewrite H7. by progress. by progress.
+          case H. by progress. by progress.
+          case H24. progress. case H25. progress. right. progress.
+          by case H; progress.
+          by rewrite /STATE_U_SLOT /PAIRING_PAIR_WITH_X_X_SLOT;
+            do 6! ((rewrite load_store_diff; first by progress); first by progress);
+            case H; progress; case H; by progress.
+          by rewrite /STATE_Z_SLOT /PAIRING_PAIR_WITH_X_X_SLOT;
+            do 6! ((rewrite load_store_diff; first by progress); first by progress);
+            case H; progress; case H; by progress.
+          by rewrite /PAIRING_PAIR_WITH_GENERATOR_X_SLOT /PAIRING_PAIR_WITH_X_X_SLOT;
+            do 6! ((rewrite load_store_diff; first by progress); first by progress);
+            case H; progress; case H; by progress.
+          by rewrite /PAIRING_PAIR_WITH_GENERATOR_Y_SLOT /PAIRING_PAIR_WITH_X_X_SLOT;
+            do 6! ((rewrite load_store_diff; first by progress); first by progress);
+            case H; progress; case H; by progress.
+          by rewrite /PAIRING_BUFFER_POINT_X_SLOT /PAIRING_PAIR_WITH_X_X_SLOT;
+            do 6! ((rewrite load_store_diff; first by progress); first by progress);
+            case H; progress; case H; by progress.
+          by rewrite /PAIRING_BUFFER_POINT_Y_SLOT /PAIRING_PAIR_WITH_X_X_SLOT;
+            do 6! ((rewrite load_store_diff; first by progress); first by progress);
+            case H; progress; case H; by progress.
+          rewrite load_store_diff.
+            by rewrite /PAIRING_PAIR_WITH_X_X_SLOT; progress.
+            by rewrite /PAIRING_PAIR_WITH_X_X_SLOT; progress.
+          rewrite load_store_same /F_to_int_point W256.of_uintK pmod_small.
+            progress. exact FieldQ.ge0_asint.
+            apply (int_lt_lt_trans _ FieldQ.p). exact FieldQ.gtp_asint. rewrite -Constants.q_eq_fieldq_p /Constants.Q. by trivial. by progress.
+          rewrite load_store_same /F_to_int_point W256.of_uintK pmod_small.
+            progress. exact FieldQ.ge0_asint.
+            apply (int_lt_lt_trans _ FieldQ.p). exact FieldQ.gtp_asint. rewrite -Constants.q_eq_fieldq_p /Constants.Q. by trivial. by progress.
+          by rewrite /PROOF_OPENING_PROOF_AT_Z_X_SLOT /PAIRING_PAIR_WITH_X_X_SLOT;
+            do 6! ((rewrite load_store_diff; first by progress); first by progress);
+            case H; progress; case H; by progress.
+          by rewrite /PROOF_OPENING_PROOF_AT_Z_Y_SLOT /PAIRING_PAIR_WITH_X_X_SLOT;
+            do 6! ((rewrite load_store_diff; first by progress); first by progress);
+            case H; progress; case H; by progress.
+          by rewrite /PROOF_OPENING_PROOF_AT_Z_OMEGA_X_SLOT /PAIRING_PAIR_WITH_X_X_SLOT;
+            do 6! ((rewrite load_store_diff; first by progress); first by progress);
+            case H; progress; case H; by progress.
+          by rewrite /PROOF_OPENING_PROOF_AT_Z_OMEGA_Y_SLOT /PAIRING_PAIR_WITH_X_X_SLOT;
+            do 6! ((rewrite load_store_diff; first by progress); first by progress);
+            case H; progress; case H; by progress.
+          by rewrite /VK_RECURSIVE_FLAG_SLOT /PAIRING_PAIR_WITH_X_X_SLOT;
+            do 6! ((rewrite load_store_diff; first by progress); first by progress);
+            case H; progress; case H; by progress.
+          by rewrite /PROOF_RECURSIVE_PART_P1_X_SLOT /PAIRING_PAIR_WITH_X_X_SLOT;
+            do 6! ((rewrite load_store_diff; first by progress); first by progress);
+            case H; progress; case H; by progress.
+          by rewrite /PROOF_RECURSIVE_PART_P1_Y_SLOT /PAIRING_PAIR_WITH_X_X_SLOT;
+            do 6! ((rewrite load_store_diff; first by progress); first by progress);
+            case H; progress; case H; by progress.
+          by rewrite /PROOF_RECURSIVE_PART_P2_X_SLOT /PAIRING_PAIR_WITH_X_X_SLOT;
+            do 6! ((rewrite load_store_diff; first by progress); first by progress);
+            case H; progress; case H; by progress.
+          by rewrite /VK_RECURSIVE_FLAG_SLOT /PAIRING_PAIR_WITH_X_X_SLOT;
+          by rewrite /PROOF_RECURSIVE_PART_P2_Y_SLOT /PAIRING_PAIR_WITH_X_X_SLOT;
+            do 6! ((rewrite load_store_diff; first by progress); first by progress);
+            case H; progress; case H; by progress.
+          by case H; progress.
+          by case H; progress.
+          by case H; progress.
+          by case H; progress.
+          by case H; progress.
+          by case H; progress.
+          by case H; progress.
+          by case H; progress.
+          exact F_to_int_point_1_ge_zero.
+          exact F_to_int_point_1_lt_p.
+          exact F_to_int_point_2_ge_zero.
+          exact F_to_int_point_2_lt_p.
+          by case H; progress.
+          by case H; progress.
+          by case H; progress.
+          by case H; progress.
+          by case H; progress.
+          by case H; progress.
+          by case H; progress.
+          by case H; progress.
+          by case H; progress.
+          by case H; progress.
+          by case H; progress.
+          by case H; progress.
+          by case H; progress.
+          by case H; progress.
+          by case H; progress.
+          by case H; progress.
+          by case H; progress.
+          by case H; progress.
+          by case H; progress.
+          by progress. by progress.
+
+          rcondf{2} 1. by progress.
+          inline Primops.mload. sp. rcondf{1} 1. progress. skip. progress. case H. by progress. by progress.
+          skip. by progress.
+
+          case (Primops.reverted{1}).
+          conseq (_ : (Primops.reverted{1} /\ failed{2}) ==> (Primops.reverted{1} /\ failed{2})).
+          progress. by case H; progress.
+          progress. case H. progress. rewrite H1 H2. reflexivity.
+          by progress.
+          seq 18 0: #pre.
+          call{1} ConcretePrimops.staticcall_pspec_revert.
+          inline*. wp. skip. by progress.
+          case (bool_of_uint256 (PurePrimops.iszero success{1})).
+          rcondt{1} 1. by progress.
+          seq 1 0: #pre. call{1} revertWithMessage_low_pspec. skip. by progress.
+          inline Primops.mload. sp.
+          case (bool_of_uint256 (PurePrimops.iszero _50{1})).
+          rcondt{1} 1. by progress.
+          call{1} revertWithMessage_low_pspec. skip. progress. left. assumption.
+          rcondf{1} 1. by progress.
+          skip. progress. left. assumption.
+          rcondf{1} 1. by progress.
+          inline Primops.mload. sp.
+          case (bool_of_uint256 (PurePrimops.iszero _50{1})).
+          rcondt{1} 1. by progress.
+          call{1} revertWithMessage_low_pspec. skip. progress. left. assumption.
+          rcondf{1} 1. by progress.
+          skip. progress. left. assumption.
+
+          conseq (_ : (
+            !Primops.reverted{1} /\
+            !failed{2} /\
+            pairing_pair_with_generator{2}.`1 = W256.to_uint (load Primops.memory{1} PAIRING_PAIR_WITH_GENERATOR_X_SLOT) /\
+            pairing_pair_with_generator{2}.`2 = W256.to_uint (load Primops.memory{1} PAIRING_PAIR_WITH_GENERATOR_Y_SLOT) /\
+            pairing_pair_with_x{2}.`1 = W256.to_uint (load Primops.memory{1} PAIRING_PAIR_WITH_X_X_SLOT) /\
+            pairing_pair_with_x{2}.`2 = W256.to_uint (load Primops.memory{1} PAIRING_PAIR_WITH_X_Y_SLOT) /\
+            0 <= pairing_pair_with_generator{2}.`1 < FieldQ.p /\
+            0 <= pairing_pair_with_generator{2}.`2 < FieldQ.p /\
+            0 <= pairing_pair_with_x{2}.`1 < FieldQ.p /\
+            0 <= pairing_pair_with_x{2}.`2 < FieldQ.p
+          ) ==> (
+            Primops.reverted{1} = failed{2}
+          )).
+          by progress; case H; progress.
+
+          seq 18 2: (
+            !Primops.reverted{1} /\
+            failed{2} = (
+              success{1} = W256.zero \/
+              load Primops.memory{1} W256.zero = W256.zero
+            )
+          ).
+          inline Primops.mstore Primops.mload Primops.gas. sp.
+          exists* Primops.memory{1}, pairing_pair_with_generator{2}, pairing_pair_with_x{2}.
+          elim*=> memory_l pairing_pair_with_generator_r pairing_pair_with_x_r.
+          progress.
+          call{1} (
+            ConcretePrimops.staticcall_ec_pairing_pspec
+              memory_l
+              (W256.of_int pairing_pair_with_generator_r.`1, W256.of_int pairing_pair_with_generator_r.`2)
+              (W256.of_int pairing_pair_with_x_r.`1, W256.of_int pairing_pair_with_x_r.`2)
+              ((G2_ELEMENTS_0_X1, G2_ELEMENTS_0_X2), (G2_ELEMENTS_0_Y1, G2_ELEMENTS_0_Y2))
+              ((G2_ELEMENTS_1_X1, G2_ELEMENTS_1_X2), (G2_ELEMENTS_1_Y1, G2_ELEMENTS_1_Y2))
+              W256.zero
+              W256.zero
+          ).
+          skip. progress.
+          do 11! ((rewrite load_store_diff; first by progress); first by progress).
+          rewrite load_store_same H1. by progress.
+          do 10! ((rewrite load_store_diff; first by progress); first by progress).
+          rewrite load_store_same H2.
+          rewrite load_store_diff.
+            by rewrite /PAIRING_PAIR_WITH_GENERATOR_Y_SLOT; progress.
+            by rewrite /PAIRING_PAIR_WITH_GENERATOR_Y_SLOT; progress.
+            by progress.
+          do 9! ((rewrite load_store_diff; first by progress); first by progress).
+          rewrite load_store_same. reflexivity.
+          do 8! ((rewrite load_store_diff; first by progress); first by progress).
+          rewrite load_store_same. reflexivity.
+          do 7! ((rewrite load_store_diff; first by progress); first by progress).
+          rewrite load_store_same. reflexivity.
+          do 6! ((rewrite load_store_diff; first by progress); first by progress).
+          rewrite load_store_same. reflexivity.
+          do 5! ((rewrite load_store_diff; first by progress); first by progress).
+          rewrite load_store_same.
+          rewrite /PAIRING_PAIR_WITH_X_X_SLOT.
+          do 6! ((rewrite load_store_diff; first by progress); first by progress).
+          rewrite H3. by progress.
+          do 4! ((rewrite load_store_diff; first by progress); first by progress).
+          rewrite load_store_same.
+          rewrite /PAIRING_PAIR_WITH_X_Y_SLOT.
+          do 7! ((rewrite load_store_diff; first by progress); first by progress).
+          rewrite H4. by progress.
+          do 3! ((rewrite load_store_diff; first by progress); first by progress).
+          rewrite load_store_same. reflexivity.
+          do 2! ((rewrite load_store_diff; first by progress); first by progress).
+          rewrite load_store_same. reflexivity.
+          (rewrite load_store_diff; first by progress); first by progress.
+          rewrite load_store_same. reflexivity.
+          rewrite load_store_same. reflexivity.
+          case (ConcretePrimops.staticcall_ec_pairing_should_succeed
+            ((W256.of_int pairing_pair_with_generator{2}.`1),
+             (W256.of_int pairing_pair_with_generator{2}.`2))
+            ((W256.of_int pairing_pair_with_x{2}.`1),
+             (W256.of_int pairing_pair_with_x{2}.`2))
+            ((G2_ELEMENTS_0_X1, G2_ELEMENTS_0_X2),
+             (G2_ELEMENTS_0_Y1, G2_ELEMENTS_0_Y2))
+            ((G2_ELEMENTS_1_X1, G2_ELEMENTS_1_X2),
+             (G2_ELEMENTS_1_Y1, G2_ELEMENTS_1_Y2))).
+          progress.
+          have H_res: result = W256.one by smt ().
+          rewrite H0. rewrite H_res.
+          have ->: W256.one <> W256.zero by smt(@W256).
+          progress.
+          have ->: (load memory_L0 W256.zero) = ((ConcretePrimops.ecPairing_precompile_unsafe_cast
+            ((W256.of_int pairing_pair_with_generator{2}.`1),
+             (W256.of_int pairing_pair_with_generator{2}.`2))
+            ((W256.of_int pairing_pair_with_x{2}.`1),
+             (W256.of_int pairing_pair_with_x{2}.`2))
+            ((G2_ELEMENTS_0_X1, G2_ELEMENTS_0_X2),
+             (G2_ELEMENTS_0_Y1, G2_ELEMENTS_0_Y2))
+            ((G2_ELEMENTS_1_X1, G2_ELEMENTS_1_X2),
+             (G2_ELEMENTS_1_Y1, G2_ELEMENTS_1_Y2)))) by smt(load_store_same).
+          rewrite /ecPairing_precompile_unsafe_cast. simplify.
+          have ->: forall (b: bool), (uint256_of_bool b = W256.zero) = !b.
+            rewrite /uint256_of_bool. progress. case b. progress. smt (@W256). by progress.
+          congr. congr. congr. congr. congr.
+          rewrite W256.of_uintK pmod_small. progress. apply (int_lt_lt_trans _ FieldQ.p). assumption. rewrite -Constants.q_eq_fieldq_p /Constants.Q. by trivial. reflexivity.
+          rewrite W256.of_uintK pmod_small. progress. apply (int_lt_lt_trans _ FieldQ.p). assumption. rewrite -Constants.q_eq_fieldq_p /Constants.Q. by trivial. reflexivity.
+          rewrite Constants.G2_element_0_int. by progress.
+          congr.          
+          rewrite W256.of_uintK pmod_small. progress. apply (int_lt_lt_trans _ FieldQ.p). assumption. rewrite -Constants.q_eq_fieldq_p /Constants.Q. by trivial.
+          rewrite W256.of_uintK pmod_small. progress. apply (int_lt_lt_trans _ FieldQ.p). assumption. rewrite -Constants.q_eq_fieldq_p /Constants.Q. by trivial. reflexivity.          
+          rewrite Constants.G2_element_1_int. by progress.
+
+
+          progress.
+          have H_res: result = W256.zero by smt ().
+          rewrite H0. rewrite H_res.
+          progress.
+          pose pairing := ecPairing_precompile _ _.
+          have ->: pairing = None.
+            apply eq_none_of_is_none.
+            rewrite /pairing.
+            have H_none: is_none
+              (ecPairing_precompile
+                ((FieldQ.inF (W256.to_uint (W256.of_int pairing_pair_with_generator{2}.`1)),
+                 FieldQ.inF (W256.to_uint (W256.of_int pairing_pair_with_generator{2}.`2))),
+                ((FieldQ.inF (W256.to_uint (W256.of_int Constants.G2_ELEMENT_0.`1.`1)),
+                 FieldQ.inF (W256.to_uint (W256.of_int Constants.G2_ELEMENT_0.`1.`2))),
+                (FieldQ.inF (W256.to_uint (W256.of_int Constants.G2_ELEMENT_0.`2.`1)),
+                FieldQ.inF (W256.to_uint (W256.of_int Constants.G2_ELEMENT_0.`2.`2)))))
+                ((FieldQ.inF (W256.to_uint (W256.of_int pairing_pair_with_x{2}.`1)),
+                FieldQ.inF (W256.to_uint (W256.of_int pairing_pair_with_x{2}.`2))),
+                ((FieldQ.inF (W256.to_uint (W256.of_int Constants.G2_ELEMENT_1.`1.`1)),
+                FieldQ.inF (W256.to_uint (W256.of_int Constants.G2_ELEMENT_1.`1.`2))),
+                (FieldQ.inF (W256.to_uint (W256.of_int Constants.G2_ELEMENT_1.`2.`1)),
+                FieldQ.inF (W256.to_uint (W256.of_int Constants.G2_ELEMENT_1.`2.`2)))))).
+                apply (
+                  ConcretePrimops.ecPairing_precomp_is_none_of_should_not_succeed
+                    (W256.of_int pairing_pair_with_generator{2}.`1, W256.of_int pairing_pair_with_generator{2}.`2)
+                    (W256.of_int pairing_pair_with_x{2}.`1, W256.of_int pairing_pair_with_x{2}.`2)
+                    
+                      (
+                        (W256.of_int Constants.G2_ELEMENT_0.`1.`1, W256.of_int Constants.G2_ELEMENT_0.`1.`2),
+                        (W256.of_int Constants.G2_ELEMENT_0.`2.`1, W256.of_int Constants.G2_ELEMENT_0.`2.`2)
+                      )
+                      (
+                        (W256.of_int Constants.G2_ELEMENT_1.`1.`1, W256.of_int Constants.G2_ELEMENT_1.`1.`2),
+                        (W256.of_int Constants.G2_ELEMENT_1.`2.`1, W256.of_int Constants.G2_ELEMENT_1.`2.`2)
+                      )
+                    
+                ). progress.
+                rewrite W256.of_uintK pmod_small. progress. apply (int_lt_lt_trans _ FieldQ.p). assumption. rewrite -Constants.q_eq_fieldq_p /Constants.Q. by trivial. assumption.
+                rewrite W256.of_uintK pmod_small. progress. apply (int_lt_lt_trans _ FieldQ.p). assumption. rewrite -Constants.q_eq_fieldq_p /Constants.Q. by trivial. assumption.
+                rewrite W256.of_uintK pmod_small. progress. apply (int_lt_lt_trans _ FieldQ.p). assumption. rewrite -Constants.q_eq_fieldq_p /Constants.Q. by trivial. assumption.
+                rewrite W256.of_uintK pmod_small. progress. apply (int_lt_lt_trans _ FieldQ.p). assumption. rewrite -Constants.q_eq_fieldq_p /Constants.Q. by trivial. assumption.
+                rewrite -Constants.q_eq_fieldq_p /Constants.Q /Constants.G2_ELEMENT_0. by progress.
+                rewrite -Constants.q_eq_fieldq_p /Constants.Q /Constants.G2_ELEMENT_0. by progress.
+                rewrite -Constants.q_eq_fieldq_p /Constants.Q /Constants.G2_ELEMENT_0. by progress.
+                rewrite -Constants.q_eq_fieldq_p /Constants.Q /Constants.G2_ELEMENT_0. by progress.
+                rewrite -Constants.q_eq_fieldq_p /Constants.Q /Constants.G2_ELEMENT_1. by progress.
+                rewrite -Constants.q_eq_fieldq_p /Constants.Q /Constants.G2_ELEMENT_1. by progress.
+                rewrite -Constants.q_eq_fieldq_p /Constants.Q /Constants.G2_ELEMENT_1. by progress.
+                rewrite -Constants.q_eq_fieldq_p /Constants.Q /Constants.G2_ELEMENT_1. by progress.
+                rewrite Constants.G2_element_0_int.
+                rewrite Constants.G2_element_1_int. by progress.
+            do rewrite W256.of_uintK in H_none.
+            rewrite pmod_small in H_none. progress. apply (int_lt_lt_trans _ FieldQ.p). assumption. rewrite -Constants.q_eq_fieldq_p /Constants.Q. by trivial.
+            rewrite pmod_small in H_none. progress. apply (int_lt_lt_trans _ FieldQ.p). assumption. rewrite -Constants.q_eq_fieldq_p /Constants.Q. by trivial.
+            rewrite pmod_small in H_none. rewrite /Constants.G2_ELEMENT_0. by progress.
+            rewrite pmod_small in H_none. rewrite /Constants.G2_ELEMENT_0. by progress.
+            rewrite pmod_small in H_none. rewrite /Constants.G2_ELEMENT_0. by progress.
+            rewrite pmod_small in H_none. rewrite /Constants.G2_ELEMENT_0. by progress.
+            rewrite pmod_small in H_none. progress. apply (int_lt_lt_trans _ FieldQ.p). assumption. rewrite -Constants.q_eq_fieldq_p /Constants.Q. by trivial.
+            rewrite pmod_small in H_none. progress. apply (int_lt_lt_trans _ FieldQ.p). assumption. rewrite -Constants.q_eq_fieldq_p /Constants.Q. by trivial.
+            rewrite pmod_small in H_none. rewrite /Constants.G2_ELEMENT_1. by progress.
+            rewrite pmod_small in H_none. rewrite /Constants.G2_ELEMENT_1. by progress.
+            rewrite pmod_small in H_none. rewrite /Constants.G2_ELEMENT_1. by progress.
+            rewrite pmod_small in H_none. rewrite /Constants.G2_ELEMENT_1. by progress.
+          assumption.
+          by progress.
+          
+          case (success{1} = W256.zero).
+          rcondt{1} 1. progress. skip. progress. rewrite /bool_of_uint256 /iszero. progress. smt (@W256).
+          seq 1 0: (Primops.reverted{1} /\ failed{2}).
+          call{1} revertWithMessage_low_pspec. skip. by progress.
+          inline Primops.mload. sp.
+          case (bool_of_uint256 (PurePrimops.iszero _50{1})).
+          rcondt{1} 1. progress.
+          call{1} revertWithMessage_low_pspec. skip. progress. rewrite H0 H2. reflexivity.
+          rcondf{1} 1. by progress. skip. progress. rewrite H H0. reflexivity.
+          
+          rcondf{1} 1. progress. skip. progress. rewrite /iszero /bool_of_uint256 H0. by progress.
+          inline Primops.mload. sp.
+          case (bool_of_uint256 (PurePrimops.iszero _50{1})).
+          rcondt{1} 1. progress.
+          call{1} revertWithMessage_low_pspec. skip. progress. rewrite H0 H2. progress. rewrite /bool_of_uint256 /iszero in H1. smt ().
+          rcondf{1} 1. progress. skip. progress. rewrite H H0. progress. rewrite /bool_of_uint256 /iszero in H1. smt (@W256).
+qed.
+
+
+
+
